stage0/ulib/FStar.UInt.fsti
@@ -452,6 +452,14 @@ let shift_left (#n:pos) (a:uint_t n) (s:nat) : Tot (uint_t n) =
 let shift_right (#n:pos) (a:uint_t n) (s:nat) : Tot (uint_t n) =
   from_vec (shift_right_vec #n (to_vec #n a) s)
 
+(* Rotate operators *)
+
+let rotate_left (#n:pos) (a:uint_t n) (s:nat) : Tot (uint_t n) =
+  from_vec (rotate_left_vec #n (to_vec #n a) s)
+
+let rotate_right (#n:pos) (a:uint_t n) (s:nat) : Tot (uint_t n) =
+  from_vec (rotate_right_vec #n (to_vec #n a) s)
+
 (* Shift operators lemmas *)
 val shift_left_lemma_1: #n:pos -> a:uint_t n -> s:nat -> i:nat{i < n && i >= n - s} ->
   Lemma (requires True)
@@ -497,6 +505,35 @@ val shift_left_logor_lemma: #n:pos -> a:uint_t n -> b:uint_t n -> s:nat ->
 val shift_right_logor_lemma: #n:pos -> a:uint_t n -> b:uint_t n -> s:nat ->
   Lemma (requires True)
         (ensures (shift_right #n (logor #n a b) s = logor #n (shift_right #n a s) (shift_right #n b s)))
+
+(* Rotate operators lemmas *)
+
+val rotate_left_lemma: #n:pos -> a:uint_t n -> s:nat -> i:nat{i < n} ->
+  Lemma (requires True)
+        (ensures (nth (rotate_left #n a s) i = nth #n a ((i + s) % n)))
+        [SMTPat (nth (rotate_left #n a s) i)]
+
+val rotate_right_lemma: #n:pos -> a:uint_t n -> s:nat -> i:nat{i < n} ->
+  Lemma (requires True)
+        (ensures (nth (rotate_right #n a s) i = nth #n a ((i + n - (s % n)) % n)))
+
+(** Rotate left by n is identity *)
+val rotate_left_full_identity: #n:pos -> a:uint_t n ->
+  Lemma (rotate_left #n a n = a)
+  [SMTPat (rotate_left #n a n)]
+
+(** Rotate right by n is identity *)
+val rotate_right_full_identity: #n:pos -> a:uint_t n ->
+  Lemma (rotate_right #n a n = a)
+  [SMTPat (rotate_right #n a n)]
+
+(** Rotate left and right are inverses *)
+val rotate_left_right_inverse: #n:pos -> a:uint_t n -> s:nat ->
+  Lemma (rotate_right #n (rotate_left #n a s) s = a)
+
+(** Rotate right and left are inverses *)
+val rotate_right_left_inverse: #n:pos -> a:uint_t n -> s:nat ->
+  Lemma (rotate_left #n (rotate_right #n a s) s = a)
 
 
 (* Lemmas about value after shift operations *)
